Reunion

ISLPrograms.fst
@@ -19,7 +19,7 @@ while (i <= n){
 assert  (j != n);
 *)
 
-unfold let init_vars = 
+let init_vars = 
   Assign "n" (Const 1000000) `Seq`
   (Assign "i" (Const 0) `Seq`
   Assign "j" (Const 0))
@@ -33,14 +33,13 @@ let assert_stmt =
   Seq (Assume (Eq (Var "j") (Var "n"))) Error |||
   Assume (enot (Eq (Var "j") (Var "n")))
 
-unfold let prog1 =
-  init_vars `Seq`
-  Kleene loop_body `Seq`
-  Assume (ge (Var "i") (Var "n")) `Seq`
-  assert_stmt
+let prog1 =
+  (Seq init_vars
+       (Seq (Kleene loop_body)
+            (Seq (Assume (Eq (Var "i") (Var "n"))) assert_stmt)))
 
 // Estados y condiciones
-unfold let cond_false : cond =
+let cond_false : cond =
   fun _ -> false
 
 let pre_vacia : cond =
@@ -49,76 +48,43 @@ let pre_vacia : cond =
 let post_er_bug : cond =
   fun (st, _) -> st "n" == Nat 1000000 /\ st "i" == Nat 1000000 /\ st "j" == Nat 1000000
 
-unfold let mid_i (k : nat) : cond =
+let mid_i (k : nat) : cond =
   fun (st, _) -> k < 1000000 /\ st "n" == Nat 1000000 /\ st "i" == Nat (k + 1) /\ st "j" == Nat k
 
-unfold let variant (n : nat) : cond = 
+let variant (n : nat) : cond = 
   fun (st, _) -> n <= 1000000 /\ st "n" == Nat 1000000 /\ st "i" == Nat n /\ st "j" == Nat n
 
-unfold let pre_assign (k : nat) : cond = 
+let pre_assign (k : nat) : cond = 
   fun s -> variant k s /\ eval_expr s (Lt (Var "i") (Var "n")) == 0
 
-unfold let pre_assert : cond = 
+let pre_assert : cond = 
   fun s -> exists (k : nat). variant k s
 
 // Lemas auxiliares
-let lemma_p_i_consequence (k:nat{k < 1000000}) (s:state)
+let lemma_p_i_consequence (k:nat) (s:state)
   : Lemma (requires mid_i k s)
           (ensures (let st, hp = s in
                    exists st_init. pre_assign k (st_init, hp) /\
                    st "i" == Nat (eval_expr (st_init, hp) (Plus (Var "i") (Const 1))) /\
                    (forall y. y <> "i" ==> st y == st_init y))) =
   let st, hp = s in
-  let st_init = fun y -> if y = "i" then Nat k else st y in
+  let st_init = override st "i" (Nat k) in
   let s_init = (st_init, hp) in
-  
   assert (eval_expr s_init (Var "i") == k)
 
-let lemma_p_j_consequence (k:nat{k < 1000000}) (s:state)
+let lemma_p_j_consequence (k:nat) (s:state)
   : Lemma (requires variant (k + 1) s)
           (ensures (let st, hp = s in
                    exists st_init. mid_i k (st_init, hp) /\
                    st "j" == Nat (eval_expr (st_init, hp) (Plus (Var "j") (Const 1))) /\
                    (forall y. y <> "j" ==> st y == st_init y))) =
   let st, hp = s in
-  let st_init = fun y -> if y = "j" then Nat k else st y in
+  let st_init = override st "j" (Nat k) in
   let s_init = (st_init, hp) in
-
   assert (eval_expr s_init (Var "j") == k)
 
-let lemma_bounded_kleene (#variant : nat -> cond) (#bound : nat) (#p : stmt)
-  (bounded_step : (k:nat{k < bound} -> GTot (isl_triple (variant k) p (variant (k + 1)) cond_false)))
-  : GTot (isl_triple (variant 0) (Kleene p) (fun s -> exists (k:nat{k <= bound}). variant k s) cond_false) =
-  let variant_total (n:nat) : cond =
-    if n <= bound then variant n else cond_false
-  in
-
-  let total_step (n:nat) : GTot (isl_triple (variant_total n) p (variant_total (n + 1)) cond_false) =
-    if n < bound then
-      let p_b = bounded_step n in
-      ISL_Consequence (variant_total n) (variant_total (n+1)) cond_false p_b () () ()
-    else
-      let p_empty = ISL_Empty #p in
-      ISL_Consequence (variant_total n) (variant_total (n+1)) cond_false p_empty () () ()
-  in
-
-  let p_kleene = ISL_KleeneVariant #variant_total #p total_step in
-  ISL_Consequence (variant 0) (fun s -> exists (k:nat{k <= bound}). variant k s) cond_false p_kleene () () ()
-
-// Demostraciones formales
-let proof_init : isl_triple pre_vacia init_vars (variant 0) cond_false =
-  let p_n = ISL_Assign #pre_vacia "n" (Const 1000000) in
-  let p_i = ISL_Assign #_ "i" (Const 0) in
-  let p_j = ISL_Assign #_ "j" (Const 0) in
-
-  let p_ij = ISL_Seq p_i p_j in
-  let p_init = ISL_Seq p_n p_ij in
-
-  ISL_Consequence pre_vacia (variant 0) cond_false p_init () () ()
-
-let proof_loop_step (k : nat{k < 1000000}) : GTot (isl_triple (variant k) loop_body (variant (k + 1)) cond_false) =
-  let p_assume = ISL_Assume #(variant k) (Lt (Var "i") (Var "n")) in
-  let p_assumed = ISL_Consequence (variant k) (pre_assign k) cond_false p_assume () () () in
+let proof_loop_step (k : nat) : isl_triple (variant k) loop_body (variant (k + 1)) (fun _ -> false) =
+  let p_assumed = ISL_Assume #(variant k) (Lt (Var "i") (Var "n")) in
 
   let p_i_raw = ISL_Assign #(pre_assign k) "i" (Plus (Var "i") (Const 1)) in
   let _ = forall_intro (move_requires (lemma_p_i_consequence k)) in
@@ -133,13 +99,22 @@ let proof_loop_step (k : nat{k < 1000000}) : GTot (isl_triple (variant k) loop_b
   let p_raw = ISL_Seq p_assumed p_ij in
   ISL_Consequence (variant k) (variant (k + 1)) cond_false p_raw () () ()
 
-let proof_loop () : GTot (isl_triple (variant 0) (Kleene loop_body) (fun s -> exists (k:nat). variant k s) cond_false) =
-  let p_bounded = lemma_bounded_kleene #variant #1000000 #loop_body proof_loop_step in
-  ISL_Consequence (variant 0) (fun s -> exists (k:nat). variant k s) cond_false p_bounded () () ()
+let lemma_kleene : isl_triple (variant 0) (Kleene loop_body) (fun s -> exists (k:nat). variant k s) cond_false =
+  ISL_KleeneVariant #variant #loop_body proof_loop_step
 
-let proof_assert () : GTot (isl_triple pre_assert (Seq (Assume (Eq (Var "i") (Var "n"))) assert_stmt) cond_false post_er_bug) =
+// Demostraciones formales
+let proof_init : isl_triple pre_vacia init_vars (variant 0) cond_false =
+  let p_n = ISL_Assign #pre_vacia "n" (Const 1000000) in
+  let p_i = ISL_Assign #_ "i" (Const 0) in
+  let p_j = ISL_Assign #_ "j" (Const 0) in
+
+  let p_ij = ISL_Seq p_i p_j in
+  let p_init = ISL_Seq p_n p_ij in
+
+  ISL_Consequence pre_vacia (variant 0) cond_false p_init () () ()
+
+let proof_assert : isl_triple pre_assert (Seq (Assume (Eq (Var "i") (Var "n"))) assert_stmt) cond_false post_er_bug =
   let p_exit_raw = ISL_Assume #pre_assert (Eq (Var "i") (Var "n")) in
-  let _ = forall_intro (fun s -> move_requires (fun s -> assert (variant 1000000 s)) s) in
   let p_exit = ISL_Consequence pre_assert (variant 1000000) cond_false p_exit_raw () () () in
 
   let p_cond_err = ISL_Assume #(variant 1000000) (Eq (Var "j") (Var "n")) in
@@ -150,15 +125,8 @@ let proof_assert () : GTot (isl_triple pre_assert (Seq (Assume (Eq (Var "i") (Va
   let p_raw = ISL_Seq p_exit p_assert in
   ISL_Consequence pre_assert cond_false post_er_bug p_raw () () ()
 
-let proof_prog1 () : GTot (isl_triple pre_vacia
-  (Seq init_vars
-       (Seq (Kleene loop_body)
-            (Seq (Assume (Eq (Var "i") (Var "n"))) assert_stmt)))
-                 cond_false
-                 post_er_bug) =
-  let p_init = ISL_Consequence pre_vacia (variant 0) cond_false proof_init () () () in
-  let p_loop_assert = ISL_Seq (proof_loop ()) (proof_assert ()) in
-  let triple_seq = ISL_Seq p_init p_loop_assert in
+let proof_prog1 : isl_triple pre_vacia prog1 cond_false post_er_bug =
+  let triple_seq = proof_init `ISL_Seq` (lemma_kleene `ISL_Seq` proof_assert) in
   ISL_Consequence pre_vacia cond_false post_er_bug triple_seq () () ()
 
 (*
